<subsubsection xml:id="subsubsec-formation-of-quadratic-equations" xmlns:xi="http://www.w3.org/2001/XInclude">
    <title>Formation of Quadratic Equations</title>
    <axiom component="resources">
        <!-- Link to blurb -->
        <xi:include href="../../resources-blurb-subsec.ptx" />

        <sbsgroup widths="45% 45%" margins="2% 2%">
            <sidebyside>
                <p xml:id="auto_24zyttyl">
                    My learners <alert>do not have access</alert> to devices during class:                  
                </p>
                <p xml:id="auto_vrftfv19">
                    My learners <alert>have access</alert> to devices during class:
                </p>
            </sidebyside>        
            <sidebyside>
                <p xml:id="auto_m6fg76vz">
                    <dataurl source="lesson-plans/Numbers and Algebra/Quadratics Expressions and Equations 1/Without Devices PDFs/Formation of Quadratic Equations by Factorisations.pdf"> Offline lesson plan </dataurl>
                </p>
                <p xml:id="auto_cykkxxyt">
                    <dataurl source="lesson-plans/Numbers and Algebra/Quadratics Expressions and Equations 1/With Devices PDFs/Formation of Quadratic Equations by Factorisations.pdf"> Online lesson plan</dataurl>
                </p>
            </sidebyside>
            <sidebyside>
                <p xml:id="auto_a3thdjwe">
                    <dataurl source="lesson-plans/Numbers and Algebra/Quadratics Expressions and Equations 1/Without Devices PDFs/Step by step guide_Formation of Quadratic Equations by Factorisations.pdf"> Offline step-by-step guide</dataurl>
                </p>
                <p xml:id="auto_857wgty5">
                    <dataurl source="lesson-plans/Numbers and Algebra/Quadratics Expressions and Equations 1/With Devices PDFs/Step by step guide_Formation of Quadratic Equations by Factorisations.pdf"> Online step-by-step guide</dataurl>
                </p>
            </sidebyside>
        </sbsgroup>
    </axiom>
    <activity xml:id="auto_a9gzgulh">
        <p xml:id="auto_j7ejpyzu">
            <em><term>Work in Groups.</term></em>
        </p>
        <p xml:id="auto_hngn0oxq">
            <ol xml:id="auto_4x2a3sz3">
                <li xml:id="auto_668bwrmd">
                    <p xml:id="auto_b2o3nefj">Start by forming a quadratic equation using given roots.</p>
                </li>
                <li xml:id="auto_qrcovqfr">
                    <p xml:id="auto_ldun0q39">Write your equation in factorized form.</p>
                </li>
                <li xml:id="auto_0tmnjek7">
                    <p xml:id="auto_e2ivlgzy">Swap your equation with another group, solve it and find the roots.</p>
                </li>
            </ol>
        </p>
        <p xml:id="auto_ii6ebr6j">
            After completing the task, discuss these questions with the class:
            <ul xml:id="auto_xrun45m0">
                <li xml:id="auto_kdtezp5b">
                    <p xml:id="auto_s2klhwqz">How did you find the quadratic equation from the roots?</p>
                </li>
                <li xml:id="auto_phmnsv37">
                    <p xml:id="auto_vadi0z3n">What did you learn about factorization from this exercise?</p>
                </li>
                <li xml:id="auto_51f0r78c">
                    <p xml:id="auto_wehl8xhn">Did you notice any patterns when forming quadratic equations?</p>
                </li>
            </ul>
        </p>
        <p xml:id="auto_37l8juyn">
            Finally, each group will share their quadratic equation and the method used with the class.
        </p>
    </activity>

    <p xml:id="auto_6imf64pr">
        Any equation of the form <m>ax^2 + bx + c = 0</m> where <m>a, b \, \text{and} \, c</m> are constants and <m>a \neq 0</m> is known as a quadratic equation. 
        In this section, solutions of quadratic equations using the factor method is discussed.
    </p>

    <p xml:id="auto_vfxbtcgk">
        To solve a quadratic equation by factorisation, we aim to rewrite the quadratic equation in the form of:
        <md>
            <mrow>(x+p)(x+q) \amp = 0 </mrow>
        </md>
        where <m>p</m> and <m>q</m> are numbers that, when multiplied, give the product <m>c</m> (the constant term), 
        and when added, give the sum <m>b</m> (the coefficient of the middle term).
    </p>
    <p xml:id="auto_7zkyi955">
        To solve a quadratic eaquation, first ensure the equations is in the form;
        <me>
            ax^2 + bx + c = 0.
        </me>
        if not in the form rearrange, so that all terms are on one side of the equation and the equation equals zero.
    </p>
    <p xml:id="auto_5487gymw">
        Factor the quadratic expression:
        <ul xml:id="auto_ecnmjfre">
            <li xml:id="auto_7cqo1odg">
                <p xml:id="auto_timwzqvu">
                    Look for two numbers that when multiplied give <m>a \times c</m> (the coefficient of <m>x^2</m>)
                </p>
            </li>
            <li xml:id="auto_l0vhy3wq">
                <p xml:id="auto_e24zrfqs">
                    And, when added give <m>b</m> (the coefficient of the middle term).
                    <ul xml:id="auto_rjd7483v">
                        <li xml:id="auto_rwmc3atg">
                            <p xml:id="auto_skqwu6qm">
                                If the quadratic has a leading coefficient <m>a = 1</m>, 
                                you only need to find two numbers that multiply to <m>c</m> and add to <m>b</m>.
                            </p>
                        </li>
                        <li xml:id="auto_so6kljkq">
                            <p xml:id="auto_4c7gctf6">
                                If <m>a \neq 1</m>, find two numbers that multiply to <m>a \times c</m> and add to <m>b</m>.
                            </p>
                        </li>
                    </ul>
                </p>
            </li>
        </ul>
    </p>
    <p xml:id="auto_9bunswjl">
        Rewrite the middle term using these two numbers and factor by grouping, which you will have a quadratic of the form:
        <me>
            (x+p)(x+q) = 0
        </me>
    </p>

    <!--Examples-->
    <example xml:id="auto_sb6n3xk7">
        <statement>
            <p xml:id="auto_tpnaqkzu">
                
            </p>
            <p xml:id="auto_wqypz0w5">
                Solve
                <me>
                    x^2 + 6x + 8 = 0
                </me>                
            </p>
        </statement>
        <solution>
            <p xml:id="auto_4xn4po6l">
                Factoring the left hand side (L.H.S) of the equation.
                <me>
                    x^2 + 6x + 8 = 0
                </me>
                The factors are <m>2 \, \text {and} 4</m>.
            </p>
            <p xml:id="auto_kan7fsni">
                <md>
                    <mrow> \amp x^2 + 2x + 4x + 8 = 0 </mrow>
                </md>
                Now create common factors
                <md>
                    <mrow> \amp x(x + 2) + 4(x + 2) = 0 </mrow>
                </md>
                Grouping them together we have:
                <md>
                    <mrow> \amp (x + 2) + (x + 4) = 0 </mrow>
                </md>
            </p>
        </solution>
    </example>

     <example xml:id="auto_pzjprar4">
        <statement>
            <p xml:id="auto_g2r79gss">
                
            </p>
            <p xml:id="auto_vgy01h7a">
                Form a quadratic expression using the factoring method.
                <me>
                    6x^2 + 12x
                </me>
            </p>
        </statement>
        <solution>
            <p xml:id="auto_46cf4vpg">
                To form a quadratic expression using the factoring method, first set the expression equal to <m>0</m> to form a quadratic equation:
                <md>
                    <mrow> 6x^2 + 12x \amp = 0 </mrow>
                </md>
            </p>
            <p xml:id="auto_hlojg6xz">
                Remove the common factor out and form a bracket:
                <md>
                    <mrow>6x(x + 2) \amp = 0</mrow>
                </md>
            </p>
            <p xml:id="auto_rtylv1hr">
                Thus, the factored form of expression <m>6x^2 + 12x</m> is;
            </p>
            <p xml:id="auto_vgkf92ti">
               <md>
                <mrow>6x(x + 2) \amp = 0 </mrow>
               </md>
            </p>
        </solution>
     </example>

     <exercises xml:id="exercises-formations-of-quadratic-equatiors-by-factors">
        <!--Exercises-->
        <exercise xml:id="auto_xz69nsjj">
            <statement>
                <p xml:id="auto_p7jv5aud">
                    Form quadratic expression using the following expressions.
                    <ol xml:id="auto_98tpp6a8" marker="(a).">
                              <li xml:id="auto_1wu5hggt">
                                       <p xml:id="auto_2g1iq3iw">                                    
                                         <m>(x + 4)(x + 5)</m>
                                      </p>
                                </li>
                                <li xml:id="auto_cg5mwzht">
                                      <p xml:id="auto_skluz2rr">
                                         <m>(x + 3)^2</m>  
                                      </p>
                                </li>
                                <li xml:id="auto_z1pi6k35">
                                    <p xml:id="auto_wpxmd106">
                                        <m>4x^2 + 8x</m>
                                    </p>
                                </li>
                                <li xml:id="auto_wlf2r6my">
                                    <p xml:id="auto_g4sw8kl5">
                                        <m>3x^2 + 6x</m>
                                    </p>
                                </li>
                                <li xml:id="auto_424ic9l7">
                                    <p xml:id="auto_zknudzfl">
                                        <m>(p - q)(p - q)</m>                                    
                                    </p>
                                </li>
                                <li xml:id="auto_ig9285m0">
                                    <p xml:id="auto_yq4s2ed5">
                                        <m>(ax + b)(2ax - 3b)</m>                                    
                                    </p>
                                </li>
                                    <li xml:id="auto_0ldv8zp7">
                                        <p xml:id="auto_7fc9d2wg">
                                            <m>(x - 8)(x + 8)</m>
                                        </p>
                                    </li>
                                    <li xml:id="auto_wdebhyew">
                                        <p xml:id="auto_fkj5mdhw">
                                            <m>(4 - 2x)(\frac{1}{2}x + 3)</m>
                                        </p>
                                    </li>
                                    <li xml:id="auto_0grhi3bi">
                                        <p xml:id="auto_y082ed4k">
                                            <m>(5dx + 3d)(2dx - 4d)</m>
                                        </p>
                                    </li>
                                    <li xml:id="auto_ey4guvrh">
                                        <p xml:id="auto_uvy50u3w">
                                            <m>(\frac{1}{2} + x)^2</m>
                                        </p>
                                    </li>
                                    <li xml:id="auto_faah5qai">
                                        <p xml:id="auto_c07po388">
                                            <m>(\frac{1}{8} + \frac{1}{x})^2</m>
                                        </p>
                                    </li>
                    </ol>
                </p>
            </statement>
        </exercise>
    </exercises>
    <answer>
        <p>
          <ol  marker="(a)">
             <li>
                           <p>
                              To form a quadratic expression from the given expression, expand by multiplying terms in the first bracket with those in the second. Arrange as:
                             <md>
                                 <mrow> (x+4)(x+5) \amp = x(x+5) +4(x+5)</mrow>
                                 <mrow> \amp = x^2 + 5x + 4x + 20</mrow>
                                 <mrow> \amp = x^2 + 9x + 20</mrow>
                             </md>
                          </p>
             </li>
             <li>
                  <p>
                     To form a quadratic expression from the given expression,first consider that this expression is a perfect square and for this reason the bracket is multiplied by twice itself. Arrange as:
                     <md>
                        <mrow> (x+3)^2 \amp = x(x+3) +3(x+3)</mrow>
                        <mrow> \amp = x^2 + 3x + 3x + 9</mrow>
                        <mrow> \amp = x^2 + 6x + 9</mrow>
                     </md>
                  </p>
             </li>
             <li>
                   <p>
                     To form a quadratic expression from the given expression,First make the equation to be equal to <m>0</m> then write it as:
                     <md>
                        <mrow> 4x^2 + 8x \amp = 0</mrow>
                        <mrow> 4x(x + 2x) \amp = 0</mrow>
                     </md>
                  </p>
             </li>
             <li>
                <p>
                    To form a quadratic expression from the given expression,First make the equation to be equal to <m>0</m> then write it as:
                    <md>
                        <mrow> 3x^2 + 6x \amp = 0</mrow>
                        <mrow> 3x(x + 2) \amp = 0</mrow>
                    </md>  
                </p>
             </li>
             <li>
                <p>
                  To form aquadratic expression, multiply the terms in the first bracket with those in the second bracket. 
                  <md>
                     <mrow> (p-q)(p-q) \amp = p(p-q) - q(p-q)</mrow>
                     <mrow> \amp = p^2 - pq - pq + q^2 </mrow>
                     <mrow> \amp = p^2 - 2pq + q^2 </mrow>
                  </md> 
                </p>
             </li>
             <li>
                <p>
                  To form aquadratic expression, multiply the terms in the first bracket with those in the second bracket. 
                  <md>
                     <mrow> (ax + b)(2ax - 3b) \amp = ax(2ax - 3b) + b(2ax - 3b)</mrow>
                     <mrow> \amp = 2a^2x^2 - 3abx + 2abx - 3b^2 </mrow>
                     <mrow> \amp = 2a^2x^2 - abx - 3b^2 </mrow>
                   </md> 
                </p>
             </li>
             <li>
                <p>
                  To form aquadratic expression, multiply the terms in the first bracket with those in the second bracket. 
                  <md>
                     <mrow> (x - 8) (x + 8) \amp = x(x + 8) - 8(x + 8)</mrow>
                     <mrow> \amp = x^2 + 8x - 8x - 64 </mrow>
                     <mrow> \amp = x^2 - 64 </mrow>
                  </md> 
                </p>
             </li>
             <li>
                <p>
                  To form aquadratic expression, multiply the terms in the first bracket with those in the second bracket. 
                  <md>
                     <mrow> (4 - 2x) (\frac{1}{2}x + 3) \amp = 4(\frac{1}{2}x + 3) - 2x(\frac{1}{2}x + 3)</mrow>
                     <mrow> \amp = 2x + 12 - x^2 - 6x </mrow>
                     <mrow> \amp =  - x^2 - 4x + 12 </mrow>
                  </md> 
                </p>
             </li>
                 <li>
                     <p>
                     To form aquadratic expression, multiply the terms in the first bracket with those in the second bracket. 
                     <md>
                        <mrow> (5dx + 3d)(2dx - 4d) \amp = 5dx(2dx - 4d) + 3d(2dx - 4d)</mrow>
                        <mrow> \amp = 10d^2x^2 - 20d^2x + 6d^2x - 12d^2 </mrow>
                        <mrow> \amp = 10d^2x^2 - 14d^2x - 12d^2 </mrow>
                     </md> 
                     </p>
                  </li>
                  <li>
                      <p>
                         To form aquadratic expression, multiply the bracket by twice itself because it is a perfect square. 
                         <md>
                             <mrow> (\frac{1}{2} + x)^2 \amp = (\frac{1}{2} + x)(\frac{1}{2} + x) </mrow> 
                             <mrow> \amp = \frac{1}{2}(\frac{1}{2} + x) + x(\frac{1}{2} + x)</mrow> 
                             <mrow> \amp = \frac{1}{4} + \frac{1}{2}x + \frac{1}{2}x + x^2 </mrow>
                             <mrow> \amp = x^2 + x + \frac{1}{4} </mrow>
                          </md> 
                      </p>
                  </li>
                        <li>
                           <p>
                                To form aquadratic expression, multiply the bracket by twice itself because it is a perfect square. 
                                   <md>
                                     <mrow> (\frac{1}{8} + \frac{1}{x})^2 \amp = (\frac{1}{8} + \frac{1}{x})(\frac{1}{8} + \frac{1}{x}) </mrow> 
                                     <mrow> \amp = \frac{1}{8}(\frac{1}{8} + \frac{1}{x}) + \frac{1}{x}(\frac{1}{8} + \frac{1}{x})</mrow> 
                                     <mrow> \amp = \frac{1}{64} + \frac{1}{8x} + \frac{1}{8x} + \frac{1}{x^2} </mrow>
                                     <mrow> \amp = \frac{1}{x^2} + \frac{1}{4x} + \frac{1}{64} </mrow>
                                   </md> 
                            </p>
                      </li>
              </ol>  
        </p>
     </answer>
</subsubsection>